wip on order: simpler attempt defining order for the comparison function, not the sequence.

src/spec/Flutterbye.Seq.Ordered.fst
@@ -18,303 +18,33 @@
 
 module Flutterbye.Seq.Ordered
 open FStar.Seq
-open Flutterbye.Seq.Mem
+open Flutterbye.Order
 
-type cmp_t 'a = 'a -> 'a -> Tot bool
-
-private type reflexive_p (#a_t:Type) (lte:cmp_t a_t) (s:seq a_t)  =
-   forall x.
-      mem_p x s ==> b2t (lte x x)
-
-private type antisymmetric_p (#a_t:Type) (lte:cmp_t a_t) (s:seq a_t) =
-   length s = 0 \/
-   (forall (x:a_t{mem_p x s}) (y:a_t{mem_p y s}).
-      (lte x y && lte y x) <==> (y = x))
-
-private type transitive_p (#a_t:Type) (lte:cmp_t a_t) (s:seq a_t) =
-   forall x y z.
-      mem_p x s /\ mem_p y s /\ mem_p z s /\ b2t (lte x y && lte y z) ==> lte x z
-
-private type sequenced_p (#a_t:Type) (lte:cmp_t a_t) (s:seq a_t) =
-   forall (x:nat{x < length s}) (y:nat{y < length s}).
-      (x <= y) <==> (lte (index s x) (index s y))
-
-type pordered_p (#a_t:Type) (lte:cmp_t a_t) (s:seq a_t) =
-   reflexive_p lte s
-   /\ antisymmetric_p lte s
-   /\ transitive_p lte s
-   /\ sequenced_p lte s
-
-private val reflexive_loop:
-   lte:cmp_t 'a ->
-   s:seq 'a ->
-   i:nat{i <= length s /\ reflexive_p lte (slice s 0 i)} ->
-   Tot (b:bool{b2t b <==> reflexive_p lte s})
-      (decreases (length s - i))
-let rec reflexive_loop lte s i =
-   Flutterbye.Seq.Mem.slice_lemma s;
-   if i < length s then
-      let a = index s i in
-      if lte a a then
-         reflexive_loop lte s (i + 1)
-      else
-         false
-   else
-      true
-
-private type antisymmetric_inner_p (#a_t:Type) (lte:cmp_t a_t) (s:seq a_t) (a:a_t) =
-   forall x.
-      mem_p x s ==> (lte x a && lte a x <==> mem_p x s /\ a = x)
-
-private val antisymmetric_inner_loop:
-   lte:cmp_t 'a ->
-   s:seq 'a ->
-   a:'a ->
-   i:nat{i <= length s /\ antisymmetric_inner_p lte (slice s 0 i) a} ->
-   Tot (b:bool{b2t b <==> antisymmetric_inner_p lte s a})
-      (decreases (length s - i))
-let rec antisymmetric_inner_loop lte s a i =
-   Flutterbye.Seq.Mem.slice_lemma s;
-   if i < length s then
-      let a' = index s i in
-      if (a = a') = (lte a a' && lte a' a) then
-         antisymmetric_inner_loop lte s a (i + 1)
-      else
-         false
-   else
-      true
-
-private val antisymmetric_loop:
-   lte:cmp_t 'a ->
-   s:seq 'a ->
-   i:nat{i <= length s /\ antisymmetric_p lte (slice s 0 i)} ->
-   Tot (b:bool{b2t b <==> antisymmetric_p lte s})
-      (decreases (length s - i))
-let rec antisymmetric_loop lte s i =
-   Flutterbye.Seq.Mem.slice_lemma s;
-   if i < length s then
-      let a = index s i in
-      if antisymmetric_inner_loop lte s a 0 then
-         antisymmetric_loop lte s (i + 1)
-      else
-         false
-   else
-      true
-
-private type transitive_loop_z_p (#a_t:Type) (lte:cmp_t a_t) (s:seq a_t) (a_1:a_t) (a_2:a_t) =
-   forall z.
-      (mem_p z s /\ b2t (lte a_1 a_2 && lte a_2 z)) ==> lte a_1 z
-
-private val transitive_loop_z:
-   lte:cmp_t 'a ->
-   s:seq 'a ->
-   a_1:'a ->
-   a_2:'a ->
-   i:nat{i <= length s /\ transitive_loop_z_p lte (slice s 0 i) a_1 a_2} ->
-   Tot (b:bool{b2t b <==> transitive_loop_z_p lte s a_1 a_2})
-      (decreases (length s - i))
-let rec transitive_loop_z lte s a_1 a_2 i =
-   Flutterbye.Seq.Mem.slice_lemma s;
-   if i < length s then
-      let a_3 = index s i in
-      if lte a_1 a_2 && lte a_2 a_3 then
-         lte a_1 a_3 && transitive_loop_z lte s a_1 a_2 (i + 1)
-      else
-         transitive_loop_z lte s a_1 a_2 (i + 1)
-   else
-      true
-
-private type transitive_loop_yz_p
-      (#a_t:Type)
-      (lte:cmp_t a_t)
-      (s:seq a_t)
-      (a_1:a_t)
-      (i:nat{i <= length s})
-      =
-   forall y z.
-      (
-         mem_p y (slice s 0 i)
-         /\ mem_p z s
-         /\ b2t (lte a_1 y && lte y z)
-      )
-      ==> lte a_1 z
-
-private val transitive_loop_yz:
-   lte:cmp_t 'a ->
-   s:seq 'a ->
-   a_1:'a ->
-   i:nat{i <= length s /\ transitive_loop_yz_p lte s a_1 i} ->
-   Tot (b:bool{b2t b <==> transitive_loop_yz_p lte s a_1 (length s)})
-      (decreases (length s - i))
-let rec transitive_loop_yz lte s a_1 i =
-   Flutterbye.Seq.Mem.slice_lemma s;
-   if i < length s then
-      let a_2 = index s i in
-      if transitive_loop_z lte s a_1 a_2 0 then
-         transitive_loop_yz lte s a_1 (i + 1)
-      else
-         false
-   else
-      true
-
-private type transitive_loop_xyz_p
-      (#a_t:Type)
-      (lte:cmp_t a_t)
-      (s:seq a_t)
-      (i:nat{i <= length s})
-      =
-   forall x y z. (
-      mem_p x (slice s 0 i)
-      /\ mem_p y s
-      /\ mem_p z s
-      /\ b2t (lte x y && lte y z)
-   )
-   ==> lte x z
-
-private val transitive_loop_xyz:
-   lte:cmp_t 'a ->
-   s:seq 'a ->
-   i:nat{i <= length s /\ transitive_loop_xyz_p lte s i} ->
-   Tot (b:bool{b2t b <==> transitive_loop_xyz_p lte s (length s)})
-      (decreases (length s - i))
-let rec transitive_loop_xyz lte s i =
-   Flutterbye.Seq.Mem.slice_lemma s;
-   if i < length s then
-      let a_1 = index s i in
-      if transitive_loop_yz lte s a_1 0 then
-         transitive_loop_xyz lte s (i + 1)
-      else
-         false
-   else
-      true
-
-private val transitive:
-   lte:cmp_t 'a ->
-   s:seq 'a ->
-   Tot (b:bool{b2t b <==> transitive_p lte s})
-let transitive lte s =
-   transitive_loop_xyz lte s 0
-
-private type sequenced_loop2_p (#a_t:Type) (lte:cmp_t a_t) (s:seq a_t) (y:nat{y < length s}) (i:nat{i <= length s}) =
-   forall (x:nat{x < i}).
-      (x <= y) <==> (lte (index s x) (index s y))
-
-
-
-private val sequenced_loop2:
-   lte:cmp_t 'a ->
-   s:seq 'a ->
-   y:nat{y < length s} ->
-   i:nat{i <= length s /\ sequenced_loop2_p lte s y i} ->
-   Tot (b:bool{b2t b <==> sequenced_loop2_p lte s y (length s)})
-      (decreases (length s - i))
-let rec sequenced_loop2 lte s y i =
-   if i < length s then
-      begin
-         if (i <= y) = (lte (index s i) (index s y)) then
-            sequenced_loop2 lte s y (i + 1)
-         else
-            false
-      end
-   else
-      true
-
-private type sequenced_loop1_p (#a_t:Type) (lte:cmp_t a_t) (s:seq a_t) (i:nat{i <= length s}) =
-   forall (x:nat{x < length s}) (y:nat{y < i}).
-      (x <= y) <==> (lte (index s x) (index s y))
-
-private val sequenced_loop1:
-   lte:cmp_t 'a ->
-   s:seq 'a ->
-   i:nat{i <= length s /\ sequenced_loop1_p lte s i} ->
-   Tot (b:bool{b2t b <==> sequenced_loop1_p lte s (length s)})
-      (decreases (length s - i))
-let rec sequenced_loop1 lte s i =
-   if i < length s then
-      begin
-         if sequenced_loop2 lte s i 0 then
-            sequenced_loop1 lte s (i + 1)
-         else
-            false
-      end
-   else
-      true
-
-private val sequenced:
-   lte:cmp_t 'a ->
-   s:seq 'a ->
-   Tot (b:bool{b2t b <==> sequenced_p lte s})
-let rec sequenced lte s =
-   sequenced_loop1 lte s 0
-
-val pordered: lte:cmp_t 'a -> s:seq 'a -> Tot (b:bool{b2t b <==> pordered_p lte s})
-let pordered lte s =
-   reflexive_loop lte s 0
-   && antisymmetric_loop lte s 0
-   && transitive lte s
-   && sequenced lte s
+type ordered_p (#a_t:Type) (lte:compare_t a_t{partial_order_p lte}) (s:seq a_t) =
+   length s < 2
+   \/ (forall (x:nat{x < length s}) (y:nat{y < length s}).
+         ((x <= y) <==> (lte (index s x) (index s y))))
 
 abstract val slice_lemma:
-   lte:cmp_t 'a ->
-   s:seq 'a{pordered_p lte s} ->
+   lte:compare_t 'a{partial_order_p lte} ->
+   s:seq 'a{ordered_p lte s} ->
    Lemma
       (ensures
-         (forall (x:nat) (y:nat).
-            // if [x, y) describe a slice of `s`, then that slice is also partially ordered.
-            y <= length s && x <= y ==> pordered_p lte (slice s x y)))
+         // if [x, y) describe a slice of `s`, then that slice is also partially ordered.
+         (forall (x:nat) (y:nat{y < length s}).
+            x <= y ==> ordered_p lte (slice s x y)))
 let slice_lemma lte s =
    ()
 
-abstract val append_lemma_antisymmetry:
-   lte:cmp_t 'a ->
-   s_1:seq 'a{pordered_p lte s_1} ->
-   s_2:seq 'a{pordered_p lte s_2} ->
-   Lemma
-      (ensures (antisymmetric_p lte (append s_1 s_2)))
-let append_lemma_antisymmetry lte s_1 s_2 =
-   admit ()
-
-abstract val append_lemma_transitivity:
-   lte:cmp_t 'a ->
-   s_1:seq 'a{pordered_p lte s_1} ->
-   s_2:seq 'a{pordered_p lte s_2} ->
-   Lemma
-      (ensures (transitive_p lte (append s_1 s_2)))
-let append_lemma_transitivity lte s_1 s_2 =
-   admit ()
-
-abstract val append_lemma_sequencing:
-   lte:cmp_t 'a ->
-   s_1:seq 'a{pordered_p lte s_1} ->
-   s_2:seq 'a{pordered_p lte s_2} ->
-   Lemma
-      (requires (
-         // either `s_1` or `s_2` are of zero length
-         length s_1 = 0 || length s_2 = 0
-         // or the first element of `s_2` must not be less than the final element of `s_1`.
-         || lte (index s_1 (length s_1 - 1)) (index s_2 0)
-      ))
-      (ensures (sequenced_p lte (append s_1 s_2)))
-let append_lemma_sequencing lte s_1 s_2 =
-   let s' = append s_1 s_2 in
-   assert (b2t (sequenced_loop1 lte s' 0))
-
 abstract val append_lemma:
-   lte:cmp_t 'a ->
-   s_1:seq 'a{pordered_p lte s_1} ->
-   s_2:seq 'a{pordered_p lte s_2} ->
+   lte:compare_t 'a{partial_order_p lte} ->
+   s_1:seq 'a{ordered_p lte s_1} ->
+   s_2:seq 'a{ordered_p lte s_2} ->
    Lemma
-      (ensures (pordered_p lte (append s_1 s_2)))
+      (ensures (ordered_p lte (append s_1 s_2)))
 let append_lemma lte s_1 s_2 =
    if length s_1 > 0 && length s_2 > 0 then
-      begin
-         let s' = append s_1 s_2 in
-         //assert (reflexive_p lte s'); // understood
-         append_lemma_antisymmetry lte s_1 s_2;
-         append_lemma_transitivity lte s_1 s_2;
-         append_lemma_sequencing lte s_1 s_2;
-         ()
-      end
+      admit ()
    else
       ()
 
