src/spec/Flutterbye.Order.fst
@@ -1,0 +1,43 @@
+// $legal:629:
+//
+// Copyright 2016 Michael Lowell Roberts & Microsoft Research
+//
+// Licensed under the Apache License, Version 2.0 (the "License");
+// you may not use this file except in compliance with the License.
+// You may obtain a copy of the License at
+//
+//     http://www.apache.org/licenses/LICENSE-2.0
+//
+// Unless required by applicable law or agreed to in writing, software
+// distributed under the License is distributed on an "AS IS" BASIS,
+// WITHOUT WARRANTIES OR CONDITIONS OF ANY KIND, either express or implied.
+// See the License for the specific language governing permissions and
+// limitations under the License.
+//
+//,$
+
+module Flutterbye.Order
+
+type compare_t 'a = 'a -> 'a -> Tot bool
+
+private type reflexive_p (#a_t:Type) (lte:compare_t a_t) =
+   forall x. lte x x
+
+private type antisymmetric_p (#a_t:Type) (lte:compare_t a_t) =
+   forall x y. ((lte x y && lte y x) <==> (x = y))
+
+private type transitive_p (#a_t:Type) (lte:compare_t a_t) =
+   forall x y z. ((lte x y && lte y z) ==> lte x z)
+
+private type total_p (#a_t:Type) (lte:compare_t a_t) =
+   forall x y. (lte x y || lte y x)
+
+type partial_order_p (#a_t:Type) (lte:compare_t a_t) =
+   reflexive_p lte /\ antisymmetric_p lte /\ transitive_p lte
+
+type total_order_p (#a_t:Type) (lte:compare_t a_t) =
+   partial_order_p lte /\ total_p lte
+
+
+
+
